reduction to BinaryPR for instances satisfying the syntactic constraints; changes to definition of PR, FlatPR (additional syntactic constraints)

theories/L/Complexity/Cook/FlatPR.v
@@ -15,14 +15,94 @@ Record FlatPR := {
   }.
 
 Definition list_ofFlatType (l : list nat) ( k : nat) := forall a, a el l -> a < k.
+
+Lemma list_ofFlatType_app (l1 l2 : list nat) (k : nat) : list_ofFlatType (l1 ++ l2) k <-> list_ofFlatType l1 k /\ list_ofFlatType l2 k. 
+Proof. 
+  split; intros; unfold list_ofFlatType in *. 
+  - setoid_rewrite in_app_iff in H. split; intros; apply H; eauto. 
+  - destruct H as (H1 & H2); setoid_rewrite in_app_iff; intros a [ | ]; eauto. 
+Qed. 
+
 Definition PRWin_ofFlatType (win : PRWin nat) (k : nat) := list_ofFlatType (prem win) k /\ list_ofFlatType (conc win) k. 
 
 Definition FlatPR_wellformed fpr := 
   width fpr > 0 
+  /\ offset fpr > 0 
+  /\ (exists k, k > 0 /\ width fpr = k * offset fpr)
+  (*/\ (offset fpr <= width fpr)*)
+  /\ length (init fpr) >= width fpr
   /\ (forall win, win el windows fpr -> PRWin_of_size win (width fpr)) 
   /\ (exists k, length (init fpr) = k * offset fpr)
   /\ list_ofFlatType (init fpr) (Sigma fpr)
   /\ (forall s, s el final fpr -> list_ofFlatType s (Sigma fpr))
   /\ (forall win, win el windows fpr -> PRWin_ofFlatType win (Sigma fpr)). 
 
-Definition FlatPRLang (C : FlatPR) := FlatPR_wellformed C /\ exists (sf : list nat), list_ofFlatType sf (Sigma C) /\ relpower (valid (offset C) (width C) (windows C)) (steps C) (init C) sf /\ satFinal (final C) sf.
+Section fixParams. 
+  Variable (Sigma : nat).
+  Variable (offset : nat). 
+  Variable (width : nat).
+  Variable (windows : list (PRWin nat)). 
+  Context (G0 : width > 0).
+
+  (*validity of a rewrite *)
+  (*we use a modified version that enforces (even in the case of vacuous rewrites which are unconstrained by the rewrite windows) that the resulting strings are strings over the finite alphabet *)
+  (*(for the non-flat version, this is already enforced by typing) *)
+  Inductive validFlat: list nat -> list nat -> Prop :=
+  | validFlatB: validFlat [] [] 
+  | validFlatSA a b u v : validFlat a b -> length a < width - offset -> list_ofFlatType u Sigma -> list_ofFlatType v Sigma -> length u = offset -> length v = offset -> validFlat (u++ a) (v++ b)
+  | validFlatS a b u v rule: validFlat a b -> list_ofFlatType u Sigma -> list_ofFlatType v Sigma -> length u = offset -> length v = offset -> rule el windows -> rewritesHead rule (u ++ a) (v ++ b) -> validFlat (u ++ a) (v ++ b). 
+
+  Lemma validFlat_length_inv a b : validFlat a b -> length a = length b. 
+  Proof.
+    induction 1. 
+    - now cbn.
+    - repeat rewrite app_length. firstorder. 
+    - repeat rewrite app_length; firstorder. 
+  Qed. 
+End fixParams. 
+
+Definition FlatPRLang (C : FlatPR) := FlatPR_wellformed C 
+  /\ exists (sf : list nat), list_ofFlatType sf (Sigma C) 
+      /\ relpower (validFlat (Sigma C) (offset C) (width C) (windows C)) (steps C) (init C) sf 
+      /\ satFinal (offset C) (length (init C)) (final C) sf.
+
+Section fixInstance.
+  Variable (fpr : FlatPR). 
+  Notation Sigma := (Sigma fpr).
+  Notation offset := (offset fpr).
+  Notation width := (width fpr).
+  Notation init := (init fpr).
+  Notation windows := (windows fpr).
+  Notation final := (final fpr).
+  Notation steps := (steps fpr). 
+
+  Context (A : FlatPR_wellformed fpr). 
+
+  Lemma validFlat_multiple_of_offset a b : validFlat Sigma offset width windows a b -> exists k, |a| = k * offset. 
+  Proof. 
+    induction 1 as [ | ? ? ? ? ? IH | ? ? ? ? ? ? IH]. 
+    - exists 0. cbn; lia. 
+    - destruct IH as (k & IH). exists (S k). now rewrite app_length. 
+    - destruct IH as (k & IH). exists (S k). now rewrite app_length. 
+  Qed. 
+
+  Lemma valid_list_ofFlatType_invariant a b : 
+    list_ofFlatType a Sigma -> validFlat Sigma offset width windows a b -> list_ofFlatType b Sigma. 
+  Proof.
+    intros H0 H. induction H. 
+    - apply H0. 
+    - apply list_ofFlatType_app in H0. apply list_ofFlatType_app. tauto. 
+    - apply list_ofFlatType_app in H0. apply list_ofFlatType_app. tauto. 
+  Qed. 
+
+  Lemma relpower_valid_list_ofFlatType_invariant steps a b: 
+    list_ofFlatType a Sigma -> relpower (validFlat Sigma offset width windows) steps a b -> list_ofFlatType b Sigma. 
+  Proof. 
+    intros. induction H0; [easy | ]. 
+    apply IHrelpower. eapply valid_list_ofFlatType_invariant, H0. apply H. 
+  Qed. 
+
+  Lemma relpower_validFlat_length_inv n a b : relpower (validFlat Sigma offset width windows) n a b -> length a = length b. 
+  Proof.  induction 1; [solve [eauto] | ]. apply validFlat_length_inv in H. congruence. Qed.
+
+End fixInstance.
