theories/L/Complexity/Cook/FlatTPR.v
@@ -16,9 +16,37 @@ Definition TPRWinP_ofFlatType (winp : TPRWinP nat) (k : nat) := winEl1 winp < k 
 Definition TPRWin_ofFlatType (win : TPRWin nat) (k : nat) := TPRWinP_ofFlatType (prem win) k /\ TPRWinP_ofFlatType (conc win) k. 
 
 Definition FlatTPR_wellformed ftpr := 
-  list_ofFlatType (init ftpr) (Sigma ftpr)
+  length (init ftpr) >= 3
+  /\ list_ofFlatType (init ftpr) (Sigma ftpr)
   /\ (forall s, s el final ftpr -> list_ofFlatType s (Sigma ftpr))
   /\ (forall win, win el windows ftpr -> TPRWin_ofFlatType win (Sigma ftpr)). 
 
-Definition FlatTPRLang (C : FlatTPR) := FlatTPR_wellformed C /\ exists (sf : list nat), list_ofFlatType sf (Sigma C) /\ relpower (valid (rewritesHeadList (windows C))) (steps C) (init C) sf /\ satFinal (final C) sf. 
+Section fixParams. 
+  Variable (Sigma : nat).
+  Variable (windows : list (TPRWin nat)). 
+  Variable (p : rewritesHeadAbstract nat). 
+
+  (*validity of a rewrite *)
+  (*we use a modified version that enforces (even in the case of vacuous rewrites which are unconstrained by the rewrite windows) that the resulting strings are strings over the finite alphabet *)
+  (*(for the non-flat version, this is already enforced by typing) *)
+  Inductive validFlat : list nat -> list nat -> Prop :=
+    | validFlatB: validFlat [] [] 
+    | validFlatSA a b x y: validFlat a b -> x < Sigma -> y < Sigma -> length a < 2 -> validFlat (x:: a) (y:: b)
+    | validFlatS a b x y : validFlat a b -> x < Sigma -> y < Sigma -> p (x::a) (y::b) -> validFlat (x::a) (y::b). 
+
+  Hint Constructors valid. 
+
+  Lemma validFlat_length_inv a b : validFlat a b -> length a = length b. 
+  Proof.
+    induction 1. 
+    - now cbn.
+    - cbn; congruence.
+    - cbn; congruence. 
+  Qed. 
+
+  Lemma relpower_validFlat_length_inv n a b : relpower validFlat n a b -> length a = length b. 
+  Proof.  induction 1; [solve [eauto] | ]. apply validFlat_length_inv in H. congruence. Qed. 
+End fixParams. 
+
+Definition FlatTPRLang (C : FlatTPR) := FlatTPR_wellformed C /\ exists (sf : list nat), list_ofFlatType sf (Sigma C) /\ relpower (validFlat (Sigma C) (rewritesHeadList (windows C))) (steps C) (init C) sf /\ satFinal (final C) sf. 
 
