theories/L/Complexity/Cook/PR_homomorphisms.v
@@ -1,0 +1,494 @@
+From PslBase Require Import Base. 
+From PslBase Require Import Vectors.Vectors. 
+From Undecidability.L.Complexity.Cook Require Import Prelim FlatPR.
+From Undecidability.L.Complexity.Cook Require BinaryPR.
+Require Import Lia.
+
+(*We define uniform homomorphisms (of strings): Given strings of the same length, they output strings of the same length.*)
+Section fixX.
+  Variable (X Y : Type). 
+
+  Definition homomorphism (h : list X -> list Y) := forall x1 x2, h (x1 ++ x2) = h x1 ++ h x2. 
+
+  Lemma homo_nil h : homomorphism h -> h [] = []. 
+  Proof. 
+    intros. unfold homomorphism in H. specialize (H [] []). 
+    cbn in H; rewrite H. destruct (h []) eqn:Heqn; cbn; [ congruence | ].  
+    assert (|y :: l| = |(y :: l) ++ y :: l|) as H0 by congruence. 
+    cbn in H0. rewrite app_length in H0. cbn in H0; lia. 
+  Qed. 
+
+  Lemma homo_cons h x l : homomorphism h -> h (x::l) = h [x] ++ h l.
+  Proof. 
+    intros. replace (x :: l) with ([x] ++ l) by now cbn. apply H. 
+  Qed.
+
+  Lemma homo_concat h : homomorphism h -> forall x, h (concat x) = concat (map h x). 
+  Proof. 
+    intros. induction x. 
+    - cbn. apply homo_nil, H. 
+    - cbn. rewrite H. now rewrite IHx. 
+  Qed. 
+
+  (*the last condition excludes the trivial homomorphism x ↦ ε *)
+  Definition uniform_homomorphism (h : list X -> list Y) := homomorphism h /\ (forall x y, |h [x]| = |h [y]|) /\ (forall x, |h[x]| >= 1).
+
+  Lemma unif_homo_length h x y : uniform_homomorphism h -> |x| = |y| -> |h x| = |h y|. 
+  Proof. 
+    intros (H1 & H2 & _). 
+    revert y. induction x; intros. 
+    - destruct y; cbn in *; [ | congruence]. now cbn. 
+    - destruct y; cbn in *; [ congruence | ]. 
+      replace (a :: x) with ([a] ++ x) by now cbn. replace (x0 :: y) with ([x0] ++ y) by now cbn. 
+      rewrite !H1. rewrite !app_length. erewrite H2 with (y := x0). 
+      rewrite IHx with (y := y); eauto. 
+  Qed. 
+End fixX. 
+
+(*for natural numbers, we define bounded injectivity *)
+(*note that we only require that one of the arguments is surely bounded*)
+Definition bounded_injectivity (Y : Type) k (f : nat -> Y) := forall n1 n2, n1 < k -> f n1 = f n2 -> n1 = n2. 
+
+(*We show that we can apply a uniform homomorphism to a FlatPR instance if the homomorphism is injective on its alphabet *)
+Section fixInstance.  
+  Variable (h : list nat -> list bool).
+
+  Variable (fpr : FlatPR). 
+
+  Notation Sigma := (Sigma fpr).
+  Notation offset := (offset fpr).
+  Notation width := (width fpr).
+  Notation init := (init fpr).
+  Notation windows := (windows fpr).
+  Notation final := (final fpr).
+  Notation steps := (steps fpr). 
+
+  (*Context (A0 : FlatPR_wellformed fpr). *)
+
+  
+  Context (A1 : uniform_homomorphism h). 
+  Definition hsingle x := h [x]. 
+  Context (A2 : bounded_injectivity Sigma hsingle). 
+  Context (A3 : Sigma > 0). 
+
+  Lemma h_nil_cons x l : not (|h []| = |h (x :: l)|). 
+  Proof. 
+    intros H. replace (x ::l) with ([x] ++ l) in H by now cbn.
+    rewrite (proj1 A1) in H. rewrite (homo_nil (proj1 A1)) in H. 
+    rewrite app_length in H. cbn in H. specialize (proj2 (proj2 A1) x). lia.
+  Qed. 
+
+  Lemma h_length_inv l1 l2 : |h l1| = |h l2| -> |l1| = |l2|. 
+  Proof. 
+    revert l2. induction l1; intros. 
+    + destruct l2; [easy | now apply h_nil_cons in H].  
+    + destruct l2; [ symmetry in H; now apply h_nil_cons in H | ]. 
+      cbn. f_equal. apply IHl1. 
+      rewrite homo_cons in H; [ | apply A1]. 
+      rewrite homo_cons with (x := n) in H; [ | apply A1].
+      rewrite !app_length in H.
+      rewrite (proj1 (proj2 A1)) with (y := n) in H. lia. 
+  Qed. 
+
+  Lemma h_length_inv' l1 l2 : h l1 = h l2 -> |l1| = |l2|. 
+  Proof.  intros; now apply h_length_inv. Qed. 
+
+  Lemma h_bounded_injective l1 l2 : list_ofFlatType l1 Sigma -> h l1 = h l2 -> l1 = l2. 
+  Proof. 
+    destruct A1 as (A4 & A5). revert l2. induction l1; intros l2 H1 H0. 
+    - destruct l2; cbn in *; [ reflexivity | apply h_length_inv' in H0; cbn in H0; congruence]. 
+    - destruct l2; cbn in *; [apply h_length_inv' in H0; cbn in H0; congruence | ].  
+      rewrite homo_cons in H0; [ | apply A1]. rewrite homo_cons with (x := n) in H0; [ | apply A1]. 
+      apply app_eq_length in H0 as (H0 & H0'); [ | apply A5].
+      apply A2 in H0 as ->; [ | now apply H1 ].  
+      assert (list_ofFlatType l1 Sigma) as G1. { intros x H5. apply (H1 x (or_intror H5)). }
+      now rewrite (IHl1 l2 G1 H0'). 
+  Qed. 
+
+  Definition k := |h [0]|. 
+  Lemma h_multiplier : forall x, |h x| = k * |x|. 
+  Proof. 
+    destruct Sigma eqn:H; [lia | ].
+    unfold k. intros x. 
+    induction x; cbn. 
+    - rewrite homo_nil; cbn; [ lia | apply A1].
+    - rewrite homo_cons; [ | apply A1]. rewrite app_length. rewrite IHx. 
+      rewrite Nat.mul_succ_r. rewrite (proj1 (proj2 A1)) with (y := 0). lia. 
+  Qed. 
+
+  Lemma k_ge : k >= 1. 
+  Proof. unfold k. apply (proj2 (proj2 A1) 0). Qed. 
+
+  Lemma h_nil_inv a : h a = [] -> a = []. 
+  Proof. 
+    specialize (h_multiplier a) as H. 
+    destruct a; [ easy | ]. intros H0. 
+    rewrite H0 in H. specialize k_ge as H1. cbn in *; nia. 
+  Qed. 
+
+  Lemma h_app_inv1 a u v : h a = u ++ v -> |u| = k -> exists a1 a2, a = a1::a2 /\ h [a1] = u /\ h a2 = v. 
+  Proof. 
+    intros.  destruct a. 
+    - specialize (h_multiplier []) as H1. rewrite H in H1. rewrite app_length in H1. cbn in H1. specialize (k_ge) as H2. nia. 
+    - rewrite homo_cons in H; [ | apply A1]. 
+      specialize (h_multiplier [n]) as H1. cbn in H1. rewrite Nat.mul_1_r in H1. 
+      apply app_eq_length in H; [ | lia]. 
+      exists n, a. split;  [easy | tauto ]. 
+  Qed. 
+
+  Lemma h_app_inv a c u v : h a = u ++ v -> |u| = c * k -> exists a1 a2, a = a1 ++ a2 /\ h a1 = u /\ h a2 = v. 
+  Proof. 
+    intros. revert a u H0 H. induction c; intros. 
+    - cbn in H0; destruct u; [ | cbn in H0; congruence]. 
+      exists [], a. split; [ now cbn | split; [apply homo_nil, A1 | cbn in H; apply H]]. 
+    - cbn in H0. assert (k <= |u|) by lia. apply list_length_split1 in H1 as (s1 & s2 & H2 & H3 & ->). 
+      rewrite H0 in H3. replace (k + c * k - k) with ( c * k) in H3 by nia. 
+      rewrite <- app_assoc in H. apply h_app_inv1  in H as (a1 & a' & -> & H4 & H5); [ | apply H2] . 
+      apply IHc in H5 as (a0 & a2 & -> & H5 & H6); [ | apply H3]. 
+      exists (a1 :: a0), a2. cbn; split; [easy | split]. 
+      + rewrite homo_cons; [ | apply A1]. easy. 
+      + apply H6. 
+  Qed. 
+
+  Definition hoffset := k * offset. 
+  Definition hwidth := k * width. 
+  Definition hinit := h init. 
+  Definition hwindow win := match win with Build_PRWin prem conc => Build_PRWin (h prem) (h conc) end.
+  Definition hwindows := map hwindow windows. 
+  Definition hfinal := map h final. 
+  Definition hsteps := steps. 
+
+  Definition hBinaryPR := @BinaryPR.Build_BinaryPR hoffset hwidth hinit hwindows hfinal hsteps. 
+
+  Lemma FlatPR_homomorphism_wf : FlatPR_wellformed fpr -> BinaryPR.BinaryPR_wellformed hBinaryPR. 
+  Proof. 
+    intros (H1 & H2 & H3 & H4 & H5 & H6 & H7). split; [ | split; [ | split]]; cbn. 
+    + unfold hwidth. unfold k. specialize (proj2 (proj2 A1) 0) as H8. nia. 
+    + unfold hinit, hwidth. rewrite h_multiplier. nia. 
+    + unfold hwidth. intros [] H. unfold hwindows in H. apply in_map_iff in H as (win' & <- & H). 
+      destruct win'. apply H5 in H. destruct H as (H & H0); cbn in *. split; cbn; now rewrite h_multiplier. 
+    + destruct H6 as (k' & H6). unfold hinit, hoffset. rewrite h_multiplier, H6. exists k'. nia. 
+  Qed. 
+
+  Context (A : FlatPR_wellformed fpr). 
+
+  Lemma valid_vacuous (X : Type) width offset windows (a b : list X) m: |a| = |b| -> |a| < width -> |a| = m * offset -> valid offset width windows a b.
+  Proof. 
+    revert a b. induction m; intros.  
+    - cbn in H1. destruct a; [ | cbn in H1; congruence]. destruct b; [ | cbn in H; congruence ].  constructor. 
+    - cbn in H1. assert (offset <= |a|) by lia. apply list_length_split1 in H2 as (s1 & s2 & H3 & H4 & H5).  
+      assert (offset <= |b|) by lia. apply list_length_split1 in H2 as (s3 & s4 & H6 & H7 & H8). 
+      rewrite H5, H8. constructor 2. 
+      + subst. apply IHm. 
+        * rewrite !app_length in H. lia. 
+        * rewrite app_length in H0. lia. 
+        * rewrite app_length in *. lia. 
+      + lia. 
+      + lia. 
+      + lia.  
+  Qed. 
+
+  Lemma validFlat_vacuous Sigma width offset windows (a b : list nat) m : |a| = |b| -> |a| < width -> |a| = m * offset -> list_ofFlatType a Sigma -> list_ofFlatType b Sigma -> validFlat Sigma offset width windows a b.
+  Proof. 
+    revert a b. induction m; intros.  
+    - cbn in H1. destruct a; [ | cbn in H1; congruence]. destruct b; [ | cbn in H; congruence ].  constructor. 
+    - cbn in H1. assert (offset <= |a|) by lia. apply list_length_split1 in H4 as (s1 & s2 & H5 & H6 & H7).  
+      assert (offset <= |b|) by lia. apply list_length_split1 in H4 as (s3 & s4 & H8 & H9 & H10). 
+      subst. rewrite list_ofFlatType_app in H2, H3.  constructor 2. 
+      + subst. apply IHm. 
+        * rewrite !app_length in H. lia. 
+        * rewrite app_length in H0. lia. 
+        * rewrite app_length in *. lia. 
+        * tauto. 
+        * tauto. 
+      + lia. 
+      + tauto. 
+      + tauto. 
+      + lia. 
+      + lia.  
+  Qed. 
+
+  Lemma rewritesHead_homomorphism1 win a b : 
+    win el windows -> rewritesHead win a b -> rewritesHead (hwindow win) (h a) (h b). 
+  Proof. 
+    unfold hwindow. destruct win. intros H0 ((c1 & H1) & (c2 & H2)). 
+    subst. split; cbn; rewrite (proj1 A1); unfold prefix; eauto.
+  Qed. 
+
+  Lemma rewritesHead_homomorphism2 win a1 a2 u v: 
+    win el hwindows 
+    -> |a1| = offset 
+    -> |u| = k * offset 
+    -> rewritesHead win (h a1 ++ h a2) (u ++ v) 
+    -> exists b1, u = h b1 /\ |b1| = offset 
+        /\ rewritesHead win (h a1 ++ h a2) (h b1 ++ v). 
+  Proof. 
+    intros. destruct H2 as ((c1 & H3) & (c2 & H4)). 
+    unfold hwindows in H; apply in_map_iff in H as (win' & <- & H).  
+    destruct win'; cbn in *. 
+    destruct A as (_ & _ & (ak & A5 & ->) & _ & A4 & _). 
+    apply A4 in H as (H & H'). cbn in *. 
+    assert (|u| <= |h conc|) by (rewrite h_multiplier; nia). 
+    apply list_length_split1 in H2 as (b1' & b2' & H2 & _ & H2'). 
+    eapply h_app_inv in H2' as (b1 & b2 & -> & <- & <-); [ | rewrite H2, H1, Nat.mul_comm; reflexivity ]. 
+    rewrite (proj1 A1), <-app_assoc in H4.
+    apply app_eq_length in H4 as (-> & ->); [ | easy]. 
+    exists b1. 
+    split; [ easy | split]. 
+    - rewrite h_multiplier in H1; specialize k_ge; nia. 
+    - split; cbn. 
+      + unfold prefix. exists c1. easy. 
+      + unfold prefix. exists c2. now rewrite (proj1 A1), <- app_assoc. 
+  Qed. 
+
+  Lemma rewritesHead_homomorphism_iff win a b : 
+    win el windows -> rewritesHead win a b <-> rewritesHead (hwindow win) (h a) (h b). 
+  Proof. 
+    split; intros.
+    - now apply rewritesHead_homomorphism1.
+    - unfold hwindow in H0. destruct win. destruct H0 as ((c1 & H1) & (c2 & H2)). 
+      cbn in *. destruct A as (_ & _ & _ & _ & A4 & _ & _ & _ & A5). 
+      eapply h_app_inv in H1 as (a1 & a2 & -> & H1 & <-); [ | rewrite Nat.mul_comm; apply h_multiplier].  
+      eapply h_app_inv in H2 as (b1 & b2 & -> & H2 & <-); [ | rewrite Nat.mul_comm; apply h_multiplier]. 
+      specialize (A5 _ H) as (A5 & A6). cbn in *.
+      symmetry in H1. symmetry in H2. 
+      apply h_bounded_injective in H1 as <-; [ | apply A5]. 
+      apply h_bounded_injective in H2 as <-; [ | apply A6]. 
+      split; unfold prefix; eauto.  
+  Qed. 
+
+  Lemma rewritesHead_homomorphism_ofFlatType win a1 a2 b1 b2: win el windows -> rewritesHead (hwindow win) (h a1 ++ h a2) (h b1 ++ h b2) -> |b1| = offset -> list_ofFlatType b1 Sigma.
+  Proof. 
+    intros. 
+    rewrite <- !(proj1 A1) in H0. apply rewritesHead_homomorphism_iff in H0; [ | apply H]. 
+    destruct A as (_ & _ & (? & H4 & H5) & _ & A4 & _ & _ & _ & A5). 
+    specialize (A4 _ H) as (_ & A4).
+    specialize (A5 _ H) as (_ & A5). 
+    destruct H0 as (_ & (b1' & H0)). 
+    assert (offset <= |conc win|) as H2 by nia. 
+    apply list_length_split1 in H2 as (s1 & s2 & H2 & _ & H3). 
+    rewrite H3, <-app_assoc in H0. apply app_eq_length in H0 as (-> & ->); [ | lia ].
+    rewrite H3 in A5; apply list_ofFlatType_app in A5; tauto.
+  Qed. 
+
+  Hint Constructors valid. 
+  Hint Constructors validFlat.
+
+  Lemma valid_homomorphism1 a b : |a| >= width -> list_ofFlatType a Sigma -> validFlat Sigma offset width windows a b -> valid hoffset hwidth hwindows (h a) (h b).
+  Proof. 
+    intros H0 H. unfold hwidth, hoffset.
+    induction 1. 
+    + rewrite homo_nil; [eauto | apply A1]. 
+    + rewrite app_length in H0. nia. 
+    + apply list_ofFlatType_app in H. rewrite !(proj1 A1). destruct rule as [prem conc]. 
+      econstructor 3. 
+      * destruct (le_lt_dec width (|a|)). 
+        -- apply IHvalidFlat, H. nia. 
+        --(*we show that for this case, the whole string is covered by the rule *)
+          clear IHvalidFlat H2 H3. 
+          specialize (validFlat_multiple_of_offset H1) as (m & H1').
+          eapply valid_vacuous with (m := m). 
+          ++ rewrite !h_multiplier. apply validFlat_length_inv in H1. nia. 
+          ++ rewrite !h_multiplier. specialize k_ge. nia. 
+          ++ rewrite h_multiplier. nia. 
+      * rewrite h_multiplier. specialize k_ge. nia. 
+      * rewrite h_multiplier. specialize k_ge. nia. 
+      * unfold hwindows. apply in_map_iff. exists (Build_PRWin prem conc). split; [ | apply H6]. reflexivity. 
+      * rewrite <- !(proj1 A1). apply rewritesHead_homomorphism_iff; assumption.
+  Qed. 
+
+  Lemma valid_homomorphism2 a b' : |a| >= width -> list_ofFlatType a Sigma -> valid hoffset hwidth hwindows (h a) b' -> exists b, b' = h b /\ list_ofFlatType b Sigma /\ validFlat Sigma offset width windows a b.
+  Proof. 
+    unfold hoffset, hwidth. intros.  
+    remember (h a). revert a Heql H0 H. induction H1. 
+    - intros. symmetry in Heql. apply h_nil_inv in Heql. subst. exists []. 
+      split; [symmetry; apply homo_nil, (proj1 A1) | split; [ apply H0 | eauto] ]. 
+    - intros. clear IHvalid H3 H1 H2. symmetry in Heql.
+      eapply h_app_inv in Heql as (a1 & a2 & -> & F1 & F2); [ | rewrite Nat.mul_comm; apply H0]. 
+      rewrite <- F2, h_multiplier in H. 
+      rewrite <- F1, h_multiplier in H0. rewrite app_length in H4. specialize k_ge. nia. 
+    - intros. symmetry in Heql.  
+      eapply h_app_inv in Heql as (a1 & a2 & -> & F1 & F2); [ | rewrite Nat.mul_comm; apply H]. 
+      subst. 
+      specialize (k_ge) as F. 
+      apply rewritesHead_homomorphism2 in H3 as (b1 & -> & H7 & H3); 
+        [ | apply H2 | rewrite h_multiplier in H; specialize k_ge; nia | apply H0]. 
+      specialize (h_multiplier a1) as H6. 
+      assert (|a1| = offset) by nia. 
+      destruct (le_lt_dec width (|a2|)). 
+      + (*we can apply the IH *)
+        unfold hwindows in H2. apply in_map_iff in H2 as (rule' & <- & H10). 
+        apply list_ofFlatType_app in H4 as (H4 & H4'). 
+        assert (|a2| >= width) as l' by lia; clear l.
+        specialize (IHvalid a2 eq_refl H4' l') as (b0 & -> & IH1 & IH2). 
+        exists (b1 ++ b0). repeat split.
+        * now rewrite (proj1 A1). 
+        * apply list_ofFlatType_app. split; [ | apply IH1]. apply rewritesHead_homomorphism_ofFlatType in H3; eauto. 
+        * econstructor 3. 
+          -- apply IH2.  
+          -- apply H4.
+          -- eapply rewritesHead_homomorphism_ofFlatType; eauto.
+          -- apply H8. 
+          -- apply H7. 
+          -- apply H10. 
+          -- rewrite <- !(proj1 A1) in H3. apply rewritesHead_homomorphism_iff in H3; eauto.
+      + (*the interesting base case *)
+        clear IHvalid H6. unfold hwindows in H2. apply in_map_iff in H2 as (rule' & <- & H10). 
+        (*we show: the rule actually matches the whole string *)
+        remember H3 as H30. clear HeqH30. (*we'll need the original hypothesis later *)
+        specialize H3 as ((rest' & H3') & (rest & H3)). (*show rest = [] *)
+        (*we need some structural assumptions *)
+        destruct A as (_ & _ & A4 & _ & A6 & _ & _ & _ & A5). 
+        assert (rest = []) as ->. 
+        { 
+          assert (|a1++a2| = width). 
+          { 
+            specialize (valid_multiple_of_offset H1) as (k1 & H1').
+            rewrite app_length. destruct A4 as (ak & _ & A4). rewrite A4 in *. rewrite app_length in H5. 
+            rewrite H8 in *.  
+            rewrite h_multiplier in H1'. 
+            enough (ak = S k1) by nia. nia. 
+          }
+          clear H5 A4. 
+          specialize (A6 _ H10) as (A6 & A6'). 
+          assert (rest' = []) as ->. 
+          { (*we now know: | h(a1 ++ a2)| = k * width, but also |prem (hwindow rule')| = k * width *)
+            clear A5 l H8 H7 H4 H3. 
+            assert (|h a1 ++ h a2| = | prem (hwindow rule') ++ rest'|) by congruence. 
+            rewrite <- (proj1 A1) in H3. 
+            destruct rule' as (prem & conc); cbn in *. rewrite app_length in H3. 
+            rewrite !h_multiplier, H2, A6 in H3.  destruct rest'; cbn in H3; [easy | nia]. 
+          } 
+          enough (|h b1 ++ b| = |h a1 ++ h a2|) as H11.
+          { rewrite H3, H3' in H11. rewrite !app_length in H11. 
+            destruct rule'; cbn in *. rewrite !h_multiplier, A6, A6' in H11. 
+            destruct rest; cbn in H11; [auto | lia]. 
+          }
+          rewrite !app_length. apply valid_length_inv in H1. lia.
+        }
+        rewrite app_nil_r in H3. specialize (A5 _ H10) as (_ & A5).
+        destruct rule'; cbn in *.  
+
+        symmetry in H3. eapply h_app_inv in H3 as (b1' & b2 & -> & H3 & <-); [ | rewrite h_multiplier, Nat.mul_comm; reflexivity]. 
+        assert (b1' = b1) as -> by (apply h_bounded_injective in H3; now apply list_ofFlatType_app in A5). 
+        clear H3. 
+        (*we have now arrived at a point where we know that the conclusion is also of the form h _  *)
+        exists (b1 ++ b2). split; [now rewrite !(proj1 A1) | split; [ apply A5 | ]].
+        (*thus, we can show the validity *)
+        econstructor 3. 
+        -- specialize (valid_multiple_of_offset H1) as (k1 & H1'). eapply validFlat_vacuous.  
+           ++ apply valid_length_inv in H1. rewrite !h_multiplier in H1. nia. 
+           ++ apply l.  
+           ++ rewrite h_multiplier in H1'. enough (|a2| = k1 * offset) as G by apply G. nia. 
+           ++ apply list_ofFlatType_app in H4; apply H4. 
+           ++ apply list_ofFlatType_app in A5; apply A5. 
+        -- apply list_ofFlatType_app in H4; apply H4. 
+        -- apply list_ofFlatType_app in A5; apply A5. 
+        -- apply H8. 
+        -- apply H7. 
+        -- apply H10. 
+        -- apply rewritesHead_homomorphism_iff; [ apply H10 | rewrite !(proj1 A1); apply H30].
+  Qed. 
+
+  (*we can obtain an equivalence, but its second direction is significantly weaker than the direction which we've just shown *)
+  Lemma valid_homomorphism_iff a b : 
+    |a| >= width -> list_ofFlatType a Sigma -> validFlat Sigma offset width windows a b <-> valid hoffset hwidth hwindows (h a) (h b).
+  Proof. 
+    intros H0 H; split. unfold hwidth, hoffset. 
+    - apply valid_homomorphism1; easy.  
+    - intros. apply valid_homomorphism2 in H1 as (b' & Heq & H2 & H1). 
+      + symmetry in Heq. apply h_bounded_injective in Heq; easy. 
+      + apply H0. 
+      + apply H. 
+  Qed. 
+
+  Lemma valid_relpower_homomorphism1 a b steps : 
+    |a| >= width -> list_ofFlatType a Sigma -> relpower (validFlat Sigma offset width windows) steps a b -> relpower (valid (k * offset) (k * width) hwindows) steps (h a) (h b).
+  Proof. 
+    intros H H0. induction 1; [ eauto | ]. econstructor. 
+    + apply valid_homomorphism_iff; [ apply H |apply H0 | apply H1 ]. 
+    + apply IHrelpower. 
+      * apply validFlat_length_inv in H1. lia. 
+      * eapply valid_list_ofFlatType_invariant; eauto. 
+  Qed. 
+
+  Lemma valid_relpower_homomorphism2 a b' steps: 
+    |a| >= width -> list_ofFlatType a Sigma -> relpower (valid (k * offset) (k * width) hwindows) steps (h a) b' -> exists b, b' = h b /\ relpower (validFlat Sigma offset width windows) steps a b. 
+  Proof. 
+    intros. remember (h a). revert a Heql H H0. induction H1; intros. 
+    - exists a0. split; eauto. 
+    - subst. apply valid_homomorphism2 in H as (b' & -> & H3 & H); [ | easy | easy]. 
+      edestruct (IHrelpower b' eq_refl) as (c' & -> & IH). 
+      + apply validFlat_length_inv in H; lia. 
+      + apply H3. 
+      + exists c'; split; [ easy | ]. econstructor; easy. 
+  Qed. 
+
+  (*again a slightly weaker equivalence *)
+  Lemma valid_relpower_homomorphism_iff a b steps : 
+    |a| >= width -> list_ofFlatType a Sigma -> relpower (validFlat Sigma offset width windows) steps a b <-> relpower (valid (k * offset) (k * width) hwindows) steps (h a) (h b).
+  Proof. 
+    intros. split. 
+    - now apply valid_relpower_homomorphism1.  
+    - intros (b' & Heq & H1)%valid_relpower_homomorphism2; [ | easy | easy ]. 
+      symmetry in Heq; apply h_bounded_injective in Heq. easy. 
+      apply relpower_valid_list_ofFlatType_invariant in H1; easy. 
+  Qed. 
+
+  Lemma final_agree sf : |init| = |sf| -> satFinal offset (length init) final sf <-> satFinal hoffset (length hinit) hfinal (h sf). 
+  Proof. 
+    intros G. unfold satFinal, hoffset, hfinal. split; intros (subs & k0 & H1 & H2 & H3). 
+    - rewrite G in H2. exists (h subs), (k0). 
+      split; [now apply in_map_iff | split; [ unfold hinit; rewrite h_multiplier; nia | ]]. 
+      destruct H3 as (b & H3). rewrite <- (firstn_skipn (k0 * offset) sf). 
+      rewrite (proj1 A1). 
+      (*we make a case analysis: if subs = [], the claim holds trivially *)
+      (*otherwise, we know that sf has a length of at least k0 * offset *)
+      destruct subs. 
+      + rewrite homo_nil; [ | apply A1]. unfold prefix; cbn; eauto. 
+      + rewrite skipn_app. 
+        * rewrite H3. rewrite (proj1 A1). exists (h b); eauto. 
+        * rewrite h_multiplier. rewrite firstn_length. 
+          enough (|sf| >= k0 * offset) by nia. 
+          specialize (skipn_length (k0 * offset) sf). rewrite H3. cbn. nia. 
+    - apply in_map_iff in H1 as (subs' & <- & H1). 
+      exists subs', k0; split; [ apply H1 | ]. 
+      destruct H3 as (b & H3). unfold prefix. 
+      rewrite <- (firstn_skipn (k0 * offset) sf), (proj1 A1) in H3. 
+      unfold hinit in H2; rewrite h_multiplier in H2. split; [ specialize k_ge; nia | ]. 
+      rewrite skipn_app in H3. 
+      + eapply h_app_inv in H3 as (a1 & a2 & -> & H4 & H5); [ | rewrite Nat.mul_comm, h_multiplier; easy ].
+        exists a2. enough (a1 = subs') by easy. 
+        symmetry; apply h_bounded_injective; [ | easy].
+        destruct A as (_ & _ & _ & _ & _ & _ & _ & A8 & _). 
+        apply A8 in H1. apply H1. 
+      + rewrite h_multiplier. rewrite firstn_length. nia. 
+  Qed. 
+      
+  Lemma FlatPR_homomorphism_iff : 
+    (exists sf, list_ofFlatType sf Sigma /\ relpower (validFlat Sigma offset width windows) steps init sf /\ satFinal offset (|init|) final sf) 
+    <-> (exists sf, relpower (valid hoffset hwidth hwindows) hsteps hinit sf /\ satFinal hoffset (|hinit|) hfinal sf). 
+  Proof. 
+    unfold hsteps, hinit, hoffset, hwidth. 
+    destruct A as (_ & _ & _  & A4  & _ & _ & A5 & _). 
+    split; intros. 
+    - destruct H as (sf & H1 & H2 & H3). 
+      exists (h sf). split. 
+      + apply valid_relpower_homomorphism_iff; easy. 
+      + clear A4 A5 H1. apply final_agree. 
+        * apply relpower_validFlat_length_inv in H2. lia. 
+        * apply H3. 
+    - destruct H as (sf & H1 & H2). 
+      apply valid_relpower_homomorphism2 in H1 as (sf' & -> & H1).
+      + exists sf'. split; [ | split; [apply H1 | ]].
+        * apply relpower_valid_list_ofFlatType_invariant in H1; easy.
+        * clear A4 A5. apply final_agree. 
+          -- apply relpower_validFlat_length_inv in H1; easy. 
+          -- apply H2. 
+      + apply A4. 
+      + apply A5. 
+  Qed. 
+
+End fixInstance. 
+
+
